Add bakery problem, void LTL formulas etc

denotational/Examples.v
@@ -1,6 +1,7 @@
 From ITree Require Import
      Basics
      Subevent
+     Events.State
      Indexed.Sum.
 
 From Coq Require Import
@@ -11,6 +12,7 @@ From Coq Require Import
 
 From ExtLib Require Import
      RelDec
+     Functor
      Maps
      FMapAList
      Reducible
@@ -24,6 +26,7 @@ From Coinduction Require Import
 From CTree Require Import
      CTree
      Interp
+     Interp.State
      State
      Eq
      SBisim.
@@ -32,10 +35,11 @@ From DSL Require Import
      System
      Network
      Storage
+     Log
      Utils
      Vectors.
 
-Import CTreeNotations.
+Import CTreeNotations Log.
 Local Open Scope ctree_scope.
 Local Open Scope string_scope.
 Local Open Scope vector_scope.
@@ -49,7 +53,13 @@ Module Examples.
   Module Storage := Storage(DistrSystem).
   Import Monads Network Storage DistrSystem.
 
-  (** Some uids *)
+  (** ================================================================================ *)
+  (** This is the top-level denotation of a distributed system to a ctree of behaviors *)
+  Program Definition run{n}(v: vec n (ctree (Storage +' Net n) void)): heap -> ctree (logE heap) void :=
+    fun st: heap => run_network (Vector.map swap (run_states_log v st)).
+
+  (** ===================================================================== *)
+  (** First system, experiment -- two agents sending messages to each other *)
   Program Definition alice : uid 2 := @of_nat_lt 0 2 _.
   Program Definition bob : uid 2 := @of_nat_lt 1 2 _.
 
@@ -71,56 +81,191 @@ Module Examples.
         | Some v => store "b" (payload v)
         end).
 
-  (** Here we are evaluating two distributed systems to CTrees C1, C2.
-      We will show they are equivalent by some sort of Applicative Bisimulation
-      using the leaf equivalence below. *) 
   Definition init_heap := (List.cons ("a", 0) List.nil).
+  Definition C := run [example_alice; example_bob] init_heap.
 
-  Program Definition run{n}(v: vec n (ctree (Storage +' Net n) void)):
-    heap -> ctree (logE heap) (vec n (Task n (logE heap))) :=
-    fun st: heap => run_network (Vector.map swap (run_states v st)).
-    
-    exact (fun st: heap => run_network (X st)).
-    cbn in X.
-    Check run_network.
-    pose proof (fun st: heap => run_network (X st)).
-  Definition C1 := run_network (map voidR (Vector.map run_storage [example; example_skip] init_heap)).
-  Definition C2 := run_network (map voidR (run_storage [example_alice; example_bob] init_heap)).
+  (** ===================================================================== *)
+  (** Second system, control -- two agents without messaging *)
+  Definition example_add: ctree (Storage +' Net 2) void :=
+    daemon (
+        a <- load "a";;
+        store "b" (S (default a 0))
+      ).
 
-  Check (run_storage [example] init_heap).
-  
+  Definition example_spin: ctree (Storage +' Net 2) void :=
+    daemon (ret tt).
 
-  Definition final_heap1: heap := List.cons ("b", 1) (List.cons ("a", 0)   List.nil).
-  Definition final_heap2: heap := List.cons ("a", 0) List.nil.
+  Definition C' := run [example_add; example_spin] init_heap.
 
-  Lemma left_tree_simpl: C1 ~ Ret (Some
-                                     [(final_heap1, tt, List.nil); (final_heap2, tt, List.nil)]). 
+  Lemma correct_C_C': C ~ C'.
   Proof.
-    unfold C1, final_heap1, final_heap2, init_heap, run_storage.
-    rewrite Vector.map_map.
+    red.
+    coinduction S CIH.
+    unfold C, C'.
+    unfold example_alice, example_bob, example_add, example_spin, init_heap.
     cbn.
-    unfold run_state.
-    Search interp_state.
-    s
-    rewrite interp_state_bind.
-    cbn.
-    replace (map voidR (run_storage [example; example_skip] init_heap)) with
-      ([run_storage example init_heap; run_storage example_skip init_heap]).
-        
-    Search map.
+    unfold run, run_states, run_network.    
+    econstructor.
     
-    sb_fwd_I.
-    Check run_state.
-    time repeat (sb_fwd_I; try reflexivity).
-  Qed.
-    
-  Lemma sb_c1_c2: C1 ~ C2.
-  Proof.
-    rewrite left_tree_simpl.
-    unfold C1, C2, init_heap.
-    time repeat (sb_fwd_I; try reflexivity).
-    (**  Takes 6035.167 secs ~ 1.7h *)
-  Qed.
-    
+  Admitted.
+
 End Examples.
+
+Module Baker.
+  Module BakerSystem <: Systems.
     
+    Definition uid := fin.
+    
+    Definition uid_coerce t (a: uid t) := a.
+    Definition fin_coerce t (a: fin t) := a.
+
+    Equations reldec_uid: forall t, fin t -> fin t -> bool :=
+      reldec_uid F1 F1 := true;
+      reldec_uid (FS i) (FS j) := reldec_uid i j;
+      reldec_uid _ _ := false.
+    
+    Transparent reldec_uid.
+    
+    (** Decidable UIDs *)
+    Global Instance eqdec_uid: forall t, RelDec (@eq (uid t)) := {
+        rel_dec a b := @reldec_uid t a b
+      }.
+
+    Inductive _msg_type :=
+    | SetNumber (n: nat)
+    | GetNumber
+    | CS.
+
+    Definition msg_type := _msg_type.
+    
+    Record _store_type := { choosing : bool; number: nat }.
+
+    Definition store_type := _store_type.
+
+    Global Instance eqdec_store_type: RelDec (@eq store_type) :=
+      {|
+        rel_dec a b := andb (rel_dec (choosing a) (choosing b))
+                            (rel_dec (number a) (number b));
+      |}.
+  
+    Definition var : Set := nat.     (** binders *)
+    Definition channel(T: Type) := nat.   (** Typed channels *)
+    
+    Definition eqdec_var: RelDec (@eq var) := _.
+    Definition eqdec_channel: forall T, RelDec (@eq (channel T)) :=
+      fun T => _.
+ 
+  End BakerSystem.
+
+  Module Network := Network(BakerSystem).                               
+  Module Storage := Storage(BakerSystem).
+  Import Monads Network Storage BakerSystem.
+
+  (** ===================================================================== *)
+  (** First system, experiment -- two agents sending messages to each other *)
+  Program Definition bakery_uid : uid 4 := @of_nat_lt 0 _ _.
+  Definition to_nat{n}(f: fin n):= proj1_sig (to_nat f).
+
+  (** Do nothing, scheduler will act as a bakery *)
+  Definition bakery: ctree (stateE store_type +' Net 4) void :=
+    CTree.spinD.
+
+  (** Client participates in the bakery algorithm *)
+  Definition client: ctree (stateE store_type +' Net 4) void :=
+    daemon (
+        (* choosing[i] := 1 *)
+        p <- get;;
+        put {| choosing := true; number := p.(number) |};;
+        (* number[i] := 1 + max(number) *)
+        send bakery_uid GetNumber;;
+        (* Loop until my turn to run the critical section *)
+        CTree.iter (fun _: unit =>
+                      m <- recv;;
+                      match m with
+                      | Some (Build_Msg _ (SetNumber n)) =>
+                          put {| choosing := false; number := n |};;
+                          ret (inl tt)
+                      | Some (Build_Msg _ CS) =>
+                          (** ENTER CRITICAL SECTION!!! *)
+                          put {| choosing := false; number := 0 |};;
+                          ret (inr tt)
+                      | _ => ret (inl tt)
+                      end) tt).
+
+  Import Coq.Lists.List.ListNotations.
+  Local Open Scope fin_vector_scope.
+  
+  Notation Sys n E := (vec n (ctree E void * list (Msg n))).
+  
+  Equations schedule_one{E: Type -> Type}{n: nat}(max: nat)
+            (schedule: nat -> Sys n (Net n +' E) -> ctree E void)
+            (sys: Sys n (Net n +' E)) (r: fin n): ctree E void :=
+    schedule_one _ schedule sys r with sys $ r => {
+        schedule_one _ _ _ _ (a, q) with observe a => {
+          (* Commute branches *)
+          schedule_one _ _ _ _ _ (BrF b n' k) :=
+            Br b n' (fun i' => schedule max (sys @ r := (k i', q)));
+           
+         (* A network `send` effect, interpet it! *)
+         schedule_one _ _ _ _ _ (VisF (inl1 (Send (Build_Msg uid GetNumber))) k) :=
+           (* All messages are to the bakery, have the scheduler send the new number in reply *)
+           let msg := {| principal := uid; payload := SetNumber max |} in
+           Guard (schedule (S max) (sys @ r := (k tt, (msg :: q)%list)));
+
+         (* A network `send` that is not GetNumber does nothing. *)
+         schedule_one _ _ _ _ _ (VisF (inl1 (Send (Build_Msg _ _))) k) :=
+           Guard (schedule max (sys @ r := (k tt, q)));
+               
+         (* Receive a message *)
+         schedule_one _ _ _ _ _ (VisF (inl1 Recv) k) :=
+           (** Check my inbox q *)
+           match last q with
+           | Some msg =>
+               (** Pop the msg from the end *)
+               Guard (schedule max (sys @ r := (k (Some msg), init q)))
+            | None =>
+                (** Becomes blocked if no messages in q *)
+                Guard (schedule max (sys @ r := (Vis (inl1 Recv) k, q)))
+            end;
+
+          (* Broadcast a message to everyone not used, skip *)
+          schedule_one _ _ _ _ _ (VisF (inl1 (Broadcast b)) k) :=
+            Guard (schedule max (sys @ r := (k tt, q)));
+          
+          (* Some other downstream effect, trigger *)
+          schedule_one _ _ _ _ _ (VisF (inr1 e) k) :=
+            Guard (schedule max (sys @ r := (trigger e >>= k, q)));
+        }
+      }.
+
+    Import CTree.
+    CoFixpoint schedule{E}{n: nat}(max: nat)(sys: Sys n (Net n +' E)): ctree E void :=
+      r <- br false n ;;
+      schedule_one max schedule sys r.
+
+    Transparent schedule.
+    Transparent schedule_one.
+    Transparent vector_replace.
+
+    Lemma unfold_schedule{E}{n: nat}(max: nat)(sys: Sys n (Net n +' E)) :
+      schedule max sys ≅ (r <- br false n ;; schedule_one max schedule sys r).
+    Proof.
+      __step_equ; cbn; econstructor.
+      intros.
+      fold_subst.
+      __upto_bind_eq_equ.
+      reflexivity.
+    Qed.    
+
+  (** Evaluates Net *)
+  Program Definition run_network{E n} (s: vec n (ctree (Net n +' E) void)): ctree E void :=
+    schedule 0 (Vector.map (fun it => (it, []%list)) s).
+
+  (** ================================================================================ *)
+  (** This is the top-level denotation of a distributed system to a ctree of behaviors *)
+  Program Definition run{n}(v: vec n (ctree (stateE store_type +' Net n) void)):
+    store_type -> ctree (logE store_type) void :=
+    fun st => run_network (Vector.map swap (run_states_log v st)).
+  
+  Compute run [bakery; client; client; client] {| choosing := false; number := 0 |}.
+End Baker.
