denotational/Logic.v
@@ -1,13 +1,7 @@
-From Coq Require Import
-     String
-     Fin
-     Relations.
-
-From Equations Require Import Equations.
+From Coq Require Import Fin.
 
 From ITree Require Import
-     Indexed.Sum
-     Subevent.
+     Events.State.
 
 From CTree Require Import
      CTree
@@ -19,313 +13,188 @@ From CTree Require Import
      Core.Utils
      Interp.State.
 
+From Coinduction Require Import
+     rel coinduction tactics.
+
 From ExtLib Require Import
-     Maps
      StateMonad
-     FMapAList
-     RelDec
-     String
      Monad.
 
-From Coinduction Require Import
-     coinduction rel tactics.
-
 From DSL Require Import
-     Vectors
-     Utils
-     System.
+     System Log.
 
-Import MonadNotation SBisimNotations.
+Import Log MonadNotation SBisimNotations.
 Local Open Scope monad_scope.
-Local Open Scope string_scope.
 
 Set Implicit Arguments.
 Set Contextual Implicit.
 
-Section HSimulation.
-  
-  Context {E F: Type -> Type} {X Y : Type}.
-  Program Definition sim(RL: rel (@label E) (@label F)): mon (ctree E X -> ctree F Y -> Prop) :=
+Module HSimulation.
+  Program Definition sim{E F X Y}(RL: rel (@label E) (@label F)): mon (ctree E X -> ctree F Y -> Prop) :=
     {| body R t u :=
       forall l t', trans l t t' -> exists l', RL l l' -> exists2 u', trans l' u u' & R t' u'
     |}.
   Next Obligation.
     destruct (H0 _ _ H1).
-    exists x0. intros HL.
+    exists x0; intros HL.
     destruct (H2 HL).
     exists x1; eauto.
   Qed.
 End HSimulation.
 
-Module Shallow.
-  Module DS := DistributedSystems(DistrSystem).
-  Import DistrSystem Monad DS.
+Module Ltl.
+  Import DistrSystem Monad.
 
-  Variable (S: Type).
+  Section Param.
+    Variable (S: Type).
 
-  (** The linear temporal logic modality is encoded in the ctree,
-      the epistemic logic is reified to the Phi effect *)
-  Inductive Logic: Type -> Type :=
-  | Pred: (S -> Prop) -> Logic unit.
+    Inductive LTL: Type -> Type :=
+    | Pred: (S -> Prop) -> LTL unit.
 
-  Notation ETL := (ctree Logic unit).
-  Notation ETL' := (ctree' Logic unit).
-  
-  Definition lift(p: S -> Prop): ETL :=
-    Vis (Pred p) (fun _ => Ret tt).  
-  
-  Definition next(p: ETL): ETL :=
-    TauV p.
+    Definition lift(p: S -> Prop): ctree LTL void :=
+      Vis (Pred p) (fun _ => CTree.spinS).
 
-  CoFixpoint and_ltl(p q: ETL): ETL :=
-    match observe p, observe q with
-    | VisF (Pred p) k, VisF (Pred p') k' =>
-        Vis (Pred (fun s => p s /\ p' s))
-             (fun tt: unit => and_ltl (k tt) (k' tt))
-    | ChoiceF b n k, _ => (** distributive right *)
-        Choice b n (fun i: fin n => and_ltl (k i) q)
-    | _, ChoiceF b n k => (** distributive left *)
-        Choice b n (fun i: fin n => and_ltl p (k i))
-    | RetF _, _ => q
-    | _, RetF _ => p
-    end.
+    Definition next(p: ctree LTL void): ctree LTL void :=
+      Step p.
 
-  CoFixpoint or_ltl(p q: ETL): ETL :=
-    match observe p, observe q with
-    | VisF (Pred p) k, VisF (Pred p') k' =>
-        Vis (Pred (fun s => p s \/ p' s))
-             (fun tt: unit => or_ltl (k tt) (k' tt))
-    | ChoiceF b n k, _ => (** distributive right *)
-        Choice b n (fun i: fin n => and_ltl (k i) q)
-    | _, ChoiceF b n k => (** distributive left *)
-        Choice b n (fun i: fin n => and_ltl p (k i))
-    | RetF _, _ => q
-    | _, RetF _ => p
-    end.
-
-  Definition or_etl(p q: ETL): ETL :=
-    choiceV2 p q.
-                      
-  Definition until(p q: ETL): ETL :=
-    CTree.iter (fun _: unit =>
-                  choiceI2 
-                    (_ <- p;; Ret (inl tt))
-                    (_ <- q;; Ret (inr tt))) tt.
-
-  Definition forever(p: ETL): ETL :=
-    until p (lift (fun _ => False)).
-
-  Definition forever'(p: ETL): ETL :=
-    CTree.forever p.
-
-  (** They should be the same *)
-  Lemma forever_forever': forall p,
-      forever p ~ forever' p.
-  Proof.  
-    intros.
-    unfold sbisim.
-    coinduction ? ?.
-    unfold forever, forever', until.
-    rewrite Shallow.unfold_forever_.
-    rewrite unfold_iter; cbn.
-    cbn.
-    destruct (observe p) eqn:Hp.
-    cbn.
-    eauto; cbn.
-    eapply st_clo_bind.
-    __upto_bind_sbisim.
-    upto_bind_sbisim.
-    __upto_bind.
-    rewrite ctree_eta.
-    cbn.
-    destruct (observe p) eqn:Hp.
-    esplit.
-    apply_coinduction.
-    __coinduction_sbisim ? H.
-    __coinduction_equ ? ?.
-    esplit; [auto | cbn].
-    econstructor; cbn; intros.
-    - unfold forever, until in H.
-      rewrite unfold_iter in H.
-      cbn in H.
-      apply trans_bind_inv in H.
-      Print label.
-      inversion H.
-      destruct H.
-      Search trans.
-      eexists.
-  Admitted.
-  
-  (** Begin entailment relation on Vis states *)
-  Notation Sys R := (ctree (stateE S) R) (only parsing).
-  Notation Sys' R := (ctree' (stateE S) R) (only parsing).
-
-  Reserved Notation "a |-- b" (at level 40, left associativity).
-  Inductive entails_ {R} : Sys' R -> ETL' -> Prop :=
-  (** Visible state changes on the system match visible predicates of the logic *)
-  | PredPut: forall (p: S -> Prop) (h: S) (k: unit -> Sys R) (k': unit -> ETL),
-      p h ->
-      observe (k tt) |-- observe (k' tt) ->
-      VisF (Put h) k |-- VisF (Pred p) k'
-  (** My interpretation of 'choice' on the logic side is existential,
-      ie: I can chose which formula is satisfied by the current system.
-      This makes sense for the definition of 'p1 until p2' --
-      either p1 or p2 is satisfied but not both *)
-  | ChoiceLogic: forall n s k b,
-      (exists (i: fin n), s |-- observe (k i)) ->
-      s |-- ChoiceF b n k
-  (** Conversely, on the system side 'choice' is interpreted as 'all',
-      ie: all states of the system must be 'lawful'. *)
-  | ChoiceSystem: forall n f k b,
-      (forall (i: fin n), observe (k i) |-- f ) ->
-      ChoiceF b n k |-- f
-  (** Dont really care for 'Ret' *)
-  | RetLogic: forall t,    
-      t |-- RetF tt
-  | RetSystem: forall f r,
-      RetF r |-- f
-  where "a |-- b" := (entails_ a b).
-
-  Definition entails{R}(c: Sys R)(f: ETL): Prop :=
-    entails_ (observe c) (observe f).
-
-  Notation "a |= b" := (entails a b) (at level 40, left associativity).
-
-  Module St := Storage(DistrSystem).
-  Import St.
-
-  Definition foo : Sys unit :=
-    o <- load "a";;
-    let v := default o 0 in 
-    store "a" (v + 1).
-
-  Lemma foo_positive:
-    foo |= forever (lift (fun st => exists v, lookup "a" st = Some v /\ v > 0)).
-  Proof.
-    unfold foo, forever, until.
-    cbn.
-    Search CTree.iter.
-    Check unfold_iter.
-    rewrite unfold_iter.
-    unfold CTree.iter.
+    CoFixpoint nott(p: ctree LTL void): ctree LTL void :=
+      match observe p with
+      | VisF (Pred p) k =>
+          Vis (Pred (fun s => not (p s))) k
+      | BrF b n k =>
+          Br b n (fun i: fin n => nott (k i))
+      | RetF _ => p
+      end.
     
-    rewrite bind_bind.
-    Search iter.
-    rewrite unfold_iter.
-    cbn.
-    econstructor.
-    un
-End Test.
-  
-Module ReturnLogic.
-  CoInductive CTL s: Type :=
-  | RetL: (s -> Prop) -> CTL s
-  | NextL: CTL s -> CTL s
-  | ExistsL: CTL s -> CTL s
-  | UntilL: CTL s -> CTL s -> CTL s
-  | AndL: CTL s -> CTL s -> CTL s
-  | OrL: CTL s -> CTL s -> CTL s.
+    CoFixpoint andt(p q: ctree LTL void): ctree LTL void :=
+      match observe p, observe q with
+      | VisF (Pred p) k, VisF (Pred p') k' =>
+          Vis (Pred (fun s => p s /\ p' s))
+              (fun tt: unit => andt (k tt) (k' tt))
+      | _, VisF (Pred x) k =>
+          Vis (Pred x)
+              (fun tt: unit => andt p (k tt))
+      | VisF (Pred x) k, _ =>
+          Vis (Pred x)
+              (fun tt: unit => andt (k tt) p)
+      | BrF b n k, BrF b' n' k' => (** distributivity *)
+          BrS n (fun i: fin n =>
+                   Br (orb b b') n' (fun i': fin n' =>
+                                       andt (k i) (k' i')))
+      | RetF _, _ | _, RetF _ => lift (fun _ => False) 
+      end.
 
-  Inductive _entails {t}: ctree' void1 t -> CTL t -> Prop :=
-  | RetRet: forall (p: t -> Prop) x,
-      p x -> _entails (RetF x) (RetL p)
-  |ChoiceRet:
-    forall n k b p (i: fin n),
-      _entails (observe (k i)) (RetL p) ->
-      _entails (ChoiceF b n k) (RetL p)            
-  (** NextL: consumes visible but not invisible *)
-  | RetNext: forall x p,
-      _entails (RetF x) p ->
-      _entails (RetF x) (NextL p)
-  | ChoiceVNext: forall n k p,
-      (forall (i: fin n), _entails (observe (k i)) p) ->
-      _entails (ChoiceVF n k) (NextL p)
-  | ChoiceINext: forall n k p,
-      (forall (i: fin n), _entails (observe (k i)) (NextL p)) ->
-      _entails (ChoiceIF n k) (NextL p)
-  (** UntilL: *)
-  | ChoiceUntil: forall b n k (l r: CTL t),
-      (forall (i: fin n),
-          (_entails (observe (k i)) l /\
-             _entails (observe (k i)) (UntilL l r)) +
-            (_entails (observe (k i)) r)) ->
-      _entails (ChoiceF b n k) (UntilL l r)            
-  (** Force Until to terminate at Ret *)
-  | RetUntil: forall x l r,
-      _entails (RetF x) l \/ _entails (RetF x) r ->
-      _entails (RetF x) (UntilL l r)
-  (** ExistsL *)
-  | ChoiceExists: forall b n k p,
-      (exists (i: fin n), _entails (observe (k i)) (ExistsL p)) ->
-      _entails (ChoiceF b n k) (ExistsL p)
-  | RetExists: forall x p,
-      _entails (RetF x) p ->
-      _entails (RetF x) (ExistsL p)
-  (** AndL *)
-  | ChoiceAnd: forall n k b l r,
-      (forall (i: fin n),
-          _entails (observe (k i)) l /\
-            _entails (observe (k i)) r) ->
-      _entails (ChoiceF b n k) (AndL l r)
-  | RetAnd: forall x l r,
-      (_entails (RetF x) l) /\ (_entails (RetF x) r) ->
-      _entails (RetF x) (AndL l r)
-  (** OrL *)
-  | ChoiceOr: forall n k b l r,
-      (forall (i: fin n), _entails (observe (k i)) l \/
-                       _entails (observe (k i)) r) ->
-      _entails (ChoiceF b n k) (AndL l r)
-  | RetOr: forall x l r,
-      (_entails (RetF x) l) \/ (_entails (RetF x) r) ->
-      _entails (RetF x) (AndL l r).
+    CoFixpoint ort(p q: ctree LTL void): ctree LTL void :=
+      match observe p, observe q with
+      | VisF (Pred p) k, VisF (Pred p') k' =>
+          Vis (Pred (fun s => p s \/ p' s))
+              (fun tt: unit => ort (k tt) (k' tt))
+      | BrF b n k, BrF b' n' k' => 
+          brS2 (Br b n k)
+               (Br b' n' k')
+      | _, VisF (Pred x) k =>
+          Vis (Pred x)
+              (fun tt: unit => ort p (k tt))
+      | VisF (Pred x) k, _ =>
+          Vis (Pred x)
+              (fun tt: unit => ort (k tt) p)
+      | RetF _, _ => q
+      | _, RetF _ => p
+      end.
+    
+    (** Weak until because `p` could be true forever *)
+    Definition weak_until(p q: ctree LTL void): ctree LTL void :=
+      CTree.forever (brS2 p q).
+    
+    Definition forever(p: ctree LTL void): ctree LTL void :=
+      CTree.forever p.
 
-  Hint Constructors _entails: core.
-  Notation "A |= B" := (_entails (observe A) B)
-                         (at level 20, right associativity).
+    Definition forever'(p: ctree LTL void): ctree LTL void :=
+      weak_until p (lift (fun _ => False)).
+    
+    Definition eventually(p: ctree LTL void): ctree LTL void :=
+      nott (forever (nott p)).  
 
+    Local Arguments logE {S}.
+    (** Use the state effect as a writer monad *)
+    Inductive Rapp: @label logE -> @label LTL -> Prop :=
+    | Prp: forall (s: S) (p: S -> Prop),
+        p s ->
+        Rapp (obs (Log s) tt) (obs (Pred p) tt)
+    | Tau: Rapp tau tau.
+
+    Definition entails{X Y}: rel (ctree logE X) (ctree LTL Y) :=
+      gfp (HSimulation.sim Rapp).
+      
+  End Param.
+End Ltl.
+
+Module LtlNotations.
+  Import Ltl.
+  Notation "a |= b" := (entails a b) (at level 40, left associativity).
   (** Syntax *)
   Declare Custom Entry hprop.
-  Notation "<[ A ]>" := A (at level 99, A custom hprop).
-  Notation "s '|-' p" := (RetL (fun s => p))
-                          (in custom hprop at level 50,
-                              s constr,
-                              p constr,
-                              right associativity).
-  Notation "A /\ B" := (AndL A B)
-                        (in custom hprop at level 50,
-                            A custom hprop,
-                            B custom hprop at level 40).
-  Notation "A \/ B" := (OrL A B)
-                        (in custom hprop at level 50,
-                            A custom hprop,
-                            B custom hprop at level 40).
-  Notation "'exists' P" := (ExistsL P)
-                             (in custom hprop at level 60,
-                                 P custom hprop at level 40).
-  Notation "'next' P" := (NextL P)
-                           (in custom hprop at level 60,
-                               P custom hprop at level 40).
-  Notation "P 'until' Q" := (UntilL P Q)
+  Declare Scope hprop_scope.
+
+  Notation "<[ A ]>" := A (at level 99, A custom hprop): hprop_scope.
+  Notation "( x )" := x (in custom hprop, x at level 99) : hprop_scope.
+  Notation "x" := x (in custom hprop at level 0, x constr at level 0) : hprop_scope.
+
+  Notation "A /\ B" := (andt A B)
+                         (in custom hprop at level 50,
+                             A custom hprop,
+                             B custom hprop at level 40): hprop_scope.
+  Notation "A \/ B" := (ort A B)
+                         (in custom hprop at level 50,
+                             A custom hprop,
+                             B custom hprop at level 40): hprop_scope.
+  Notation "'○' P" := (next P)
+                        (in custom hprop at level 60,
+                            P custom hprop at level 40): hprop_scope.
+  
+  Notation "P 'U' Q" := (weak_until P Q)
                               (in custom hprop at level 60,
                                   P custom hprop,
-                                  Q custom hprop at level 40).
+                                  Q custom hprop at level 40): hprop_scope.
 
-  (** Example 1 *)
-  Definition f: CTL (nat * unit) := <[ exists n |- fst n = 1 ]>.
-  Definition t: ctree (stateE nat +' void1) unit :=
-    s <- get;;
-    choiceV2 (put 0) (put (S s));;
-    y <- get ;;
-    choiceV2 (put (S y)) (put (S (S y))).
+  Notation "'◻' P" := (forever P)
+                        (in custom hprop at level 60,
+                            P custom hprop at level 40): hprop_scope.
 
-  Lemma ex: (run_state t 0 |= f).
-    repeat (cbn; econstructor; try exists F1).
-  Defined.
+  Notation "'⋄' P" := (eventually P)
+                        (in custom hprop at level 60,
+                            P custom hprop at level 40): hprop_scope.
+End LtlNotations.
 
+(** Some scratch work and examples *)
+Import Ltl LtlNotations.
+Open Scope hprop_scope.
 
-  
-  
-End Logic.
+From DSL Require Import Utils.
+Open Scope hprop_scope.
 
+(** They should be the same *)
+Lemma forever_forever': forall (S: Type) (p: ctree (LTL S) void),
+    <[ ◻ p ]> ~ forever' p.
+Proof.  
+  intros.
+  unfold sbisim.
+  coinduction ? ?.
+  unfold forever, forever', weak_until.
+  rewrite Shallow.unfold_forever_.
+Admitted.
 
+(** Print an infinite sequence [1,1,1...] *)
+Example foo : ctree (logE nat) unit :=
+  CTree.forever (log 1).
+
+Lemma foo_positive:
+  let positive := lift (fun s => s > 0) in  
+  foo |= <[ ⋄ positive ]>.
+Proof.
+  simpl.
+  unfold entails.
+  coinduction ? ?.
+  (* Should reason equationally about LTL spec refinement *)
+Admitted.
 
