denotational/Storage.v
@@ -6,6 +6,7 @@ From Coq Require Import
 From ITree Require Import
      Indexed.Sum
      Subevent
+     Events.State
      CategoryOps.
 
 From CTree Require Import
@@ -35,10 +36,10 @@ Set Implicit Arguments.
 Module Storage(S: Systems).
   Import S Monads.
 
-  Notation heap := (alist var bytestring).
+  Notation heap := (alist var store_type).
   Notation Storage := (stateE heap).
   
-  Global Instance Map_heap: Map var bytestring heap := Map_alist eqdec_var bytestring.
+  Global Instance Map_heap: Map var store_type heap := Map_alist eqdec_var store_type.
 
   (** Equality of heaps is extensional (functional extensionality)
       for all keys in either one, values must match *)
@@ -55,38 +56,15 @@ Module Storage(S: Systems).
       andb (rec a b) (rec b a)
     }.
   
-  Definition load {E} `{stateE heap -< E}(v: var): ctree E (option bytestring) :=
+  Definition load {E} `{stateE heap -< E}(v: var): ctree E (option store_type) :=
     get >>= fun s => ret (lookup v s).
 
-  Definition store {E} `{Storage -< E}(v: var)(b: bytestring): ctree E unit :=
+  Definition store {E} `{Storage -< E}(v: var)(b: store_type): ctree E unit :=
     get >>= fun s => put (add v b s).
   
-  Section ParametricS.
-    Context {S: Type} {dec_S: RelDec (@eq S)}.
-
-    Inductive logE (S: Type): Type -> Type :=
-    | Log: S -> logE S unit.
-
-    Definition h_state_to_log {E}: stateE S ~> stateT S (ctree (logE S +' E)) :=
-      fun _ e s =>
-        match e with
-        | Get _ => Ret (s, s)
-        | Put s' => if rel_dec s s' then
-                     Ret (s, tt) else
-                     Vis (inl1 (Log s')) (fun _: unit => Ret (s', tt))
-        end.
-
-    Definition pure_state_to_log {E} : E ~> stateT S (ctree (logE S +' E))
-      := fun _ e s => Vis (inr1 e) (fun x => Ret (s, x)).
-
-    Definition run_state {E}: ctree (stateE S +' E) ~> stateT S (ctree (logE S +' E))
-      := interp_state (case_ h_state_to_log pure_state_to_log).
-
-    Definition run_states {n E R}(v: vec n (ctree (stateE S +' E) R)):
-      stateT S (fun T => vec n (ctree (logE S +' E) T)) R :=
-      fun st => Vector.map (fun a => run_state a st) v.
-    
-  End ParametricS.
+  Definition run_states {n E}(v: vec n (ctree (stateE heap +' E) void)):
+    heap -> vec n (ctree E void) :=
+    fun st => Vector.map (fun a => CTree.map snd (run_state a st)) v.  
 
 End Storage.
 
